\documentclass[12pt]{article}
\thispagestyle{empty}

\begin{document}

    S K K = I $\Longleftrightarrow$\\
    ($\lambda$ x y z.x z (y z)) ($\lambda$ x y.x) ($\lambda$ x y.x) = $\lambda$ x.x $\Longleftrightarrow$\\
    ($\lambda$ x.($\lambda$ y z.x z (y z))) ($\lambda$ x y.x)
    ($\lambda$ x y.x) = $\lambda$ x.x $\Longleftrightarrow$\\
    ($\lambda$ y z.($\lambda$ x y.x) z (y z)) ($\lambda$ x y.x)
    = $\lambda$ x.x $\Longleftrightarrow$\\
    ($\lambda$ y z.($\lambda$ y.z) (y z)) ($\lambda$ x y.x) = $\lambda$ x.x $\Longleftrightarrow$\\
    ($\lambda$ y z.z) ($\lambda$ x y.x) = $\lambda$ x.x $\Longleftrightarrow$\\
    ($\lambda$ y.$\lambda$ z.z) ($\lambda$ x y.x) = $\lambda$ x.x $\Longleftrightarrow$\\
    $\lambda$ z.z = $\lambda$ x.x $\Longleftrightarrow$\\
    I = I

\end{document}